common/Allocator.v
@@ -13,6 +13,7 @@ Require Import Tags.
 Require Export Memdata.
 Require Import Memory.
 Require Import ExtLib.Structures.Monads. Import MonadNotation.
+Require Import ExtLib.Data.Monads.OptionMonad.
 
 Open Scope monad_scope.
 
@@ -23,22 +24,6 @@ Local Unset Elimination Schemes.
 Local Unset Case Analysis Schemes.
 
 Local Notation "a # b" := (PMap.get b a) (at level 1).
-
-Notation "'do' X <- A ; B" := (match A with Some X => B | None => None end)
-  (at level 200, X name, A at level 100, B at level 200)
-  : option_monad_scope.
-
-Notation "'do' X , Y <- A ; B" := (match A with Some (X, Y) => B | None => None end)
-  (at level 200, X name, Y name, A at level 100, B at level 200)
-  : option_monad_scope.
-
-Notation "'do' X , Y , Z <- A ; B" := (match A with Some (X, Y, Z) => B | None => None end)
-  (at level 200, X name, Y name, Z name, A at level 100, B at level 200)
-  : option_monad_scope.
-
-Notation "'do' X , Y , Z , W <- A ; B" := (match A with Some (X, Y, Z, W) => B | None => None end)
-  (at level 200, X name, Y name, Z name, W name, A at level 100, B at level 200)
-  : option_monad_scope.
 
 Notation "'check' A ; B" := (if A then B else None)
   (at level 200, A at level 100, B at level 200)
@@ -219,15 +204,15 @@ Module ConcreteAllocator (P : Policy) : Allocator P.
                 (* There is enough room to split *)
                 let new := base + header_size + padded_sz in
                 let new_sz := bs - (header_size + padded_sz) in
-                do m' <- update_header m base true padded_sz vt lt;
-                do m'' <- update_header m' new false new_sz InitT DefLT;
+                m' <- update_header m base true padded_sz vt lt;;
+                m'' <- update_header m' new false new_sz InitT DefLT;;
                 (* open question: how do we (re)tag new, free headers? *) 
                 Some (m'',base)
               else
                 (* [base ][========|==][=][next] *)
                 (* [hd_sz][   sz   |/8][ ][next] *)
                 (* There is exactly enough room (or not enough extra to split) *)                
-                do m' <- update_header m base true bs vt lt;
+                m' <- update_header m base true bs vt lt;;
                 Some (m',base)
         | None => None
         end
